Progression in the proof of Structured Full Abstraction.

coq/simple-instance/SCCProof.v
@@ -26,6 +26,8 @@ Inductive neq_progH : Source.program -> Source.program -> Prop :=
     (neq_progH P P')
   where "'HIGH_NEQ' P '≁H' P'" := (neq_progH P P').
 
+(* If a[P] ≁L a[Q] we say that a distinguish the partial
+   programs P and Q. The same concept exists for ≁H *)
 
 (* _____________________________________ 
                  LEMMAS
@@ -65,23 +67,135 @@ Proof.
 Admitted.
 
 (* ------- Structured Full Abstraction ------- *)
-Theorem structured_full_abstraction :
+Definition structured_full_abstraction : Prop :=
   forall s,
   forall P Q, 
-    (PROGRAM_SHAPE P ∈• s) /\ (PROGRAM_SHAPE Q ∈• s)
-      /\
-    (program_fully_defined s P /\ program_fully_defined s Q)
+    (PROGRAM_SHAPE P ∈• s) ->
+    (PROGRAM_SHAPE Q ∈• s) ->
+    (program_fully_defined s P) ->
+    (program_fully_defined s Q) ->
+    (exists a, (LL_CONTEXT_SHAPE a ∈∘ s) /\
+       let ap := (LL_context_application a (COMPILE_PROG P↓)) in
+       let aq := (LL_context_application a (COMPILE_PROG Q↓)) in
+       LOW_NEQ ap ≁L aq)
     ->
-  forall A,
+    (exists A,
     let AP := (context_application A P) in
-    let AQ := (context_application A Q) in 
-    (CONTEXT_SHAPE A ∈∘ s) /\ (context_fully_defined s A)
-    -> HIGH_NEQ AP ≁H AQ
-    -> forall a, (LL_CONTEXT_SHAPE a ∈∘ s) ->
-        LOW_NEQ
-        (LL_context_application a (COMPILE_PROG P↓))
-          ≁L
-        (LL_context_application a (COMPILE_PROG Q↓)).
+    let AQ := (context_application A Q) in
+    (CONTEXT_SHAPE A ∈∘ s) /\ (context_fully_defined s A) ->
+    HIGH_NEQ AP ≁H AQ).
+
+Definition separate_compilation_correctness : Prop :=
+  forall s,
+  forall A P, 
+    (CONTEXT_SHAPE A ∈∘ s) ->
+    (PROGRAM_SHAPE P ∈• s) ->
+    program_fully_defined s P ->
+    context_fully_defined s A ->
+    (* 1 *)
+    ((program_terminates (context_application A P)
+    <-> cprogram_terminates (LL_context_application 
+    (COMPILE_PROG A↓) (COMPILE_PROG P↓))) 
+      /\
+    (* 2 *)
+    (program_diverges (context_application A P)
+    <-> cprogram_diverges (LL_context_application 
+    (COMPILE_PROG A↓) (COMPILE_PROG P↓)))).
+
+(* _____________________________________ 
+   SECURE COMPARTMENTALIZING COMPILATION
+            AND PROOFS OF LEMMAS
+   _____________________________________ *)
+
+Lemma shape_closed_under_compilation :
+  forall s P, PROGRAM_SHAPE P ∈• s 
+  -> LL_PROGRAM_SHAPE (COMPILE_PROG P↓) ∈• s.
+Proof.
+Admitted.
+
+Lemma trace_sets_closed_under_prefix_program :
+  forall t' t p s, (LL_PROGRAM_SHAPE p ∈• s) ->
+    incl t' t -> in_Traces_p t p s ->
+    in_Traces_p t' p s.
+Proof.
+Admitted.
+
+Lemma trace_sets_closed_under_prefix_context :
+  forall t' t a s, (LL_CONTEXT_SHAPE a ∈∘ s) ->
+    incl t' t -> in_Traces_a t a s ->
+    in_Traces_p t' a s.
+Proof.
+Admitted.
+
+Theorem structured_full_abstraction_proof :
+  structured_full_abstraction.
+Proof.
+  unfold structured_full_abstraction.
+  intros s.
+  intros P Q H_shP H_shQ H_PFD H_QFD.
+  (* We consider a ∈∘ s distinguishing P ∈• s and Q ∈• s *)
+  intros H_a. destruct H_a as [a [H_sha H_low_neq]].
+  inversion H_low_neq as [ap aq H_behavior ap_eq aq_eq].
+  (* We suppose that a[P↓] terminates and a[Q↓] diverges *)
+  destruct H_behavior as [H_behavior|H_behavior'].
+  destruct H_behavior as [ap_terminates ap_diverges].
+  (* Goal : build a full-defined A ∈∘ s such that A[P] ≁ A[Q] *)
+  (* We first apply trace decomposition *)
+  assert (H_shp := H_shP).
+  apply shape_closed_under_compilation in H_shp.
+  pose (trace_decomposition s (COMPILE_PROG P↓) 
+    H_shp a H_sha ap_terminates) as t_decomposition.
+  destruct t_decomposition as [ti H_decomposition].
+  (* We call tp the longest prefix of ti such that tp ∈ Tr•s(a) *)
+  assert 
+    (exists tp, incl tp ti /\ 
+      (in_Traces_p tp (COMPILE_PROG Q↓) s) /\
+    (forall tp', (incl tp' ti) /\ 
+      (in_Traces_p tp (COMPILE_PROG Q↓) s) ->
+      (length tp') <= (length tp) 
+    )) 
+  as tp_exists.
+  Case "Proof of existence of tp".
+  { admit. }
+  destruct tp_exists as [tp H_tp].
+  destruct H_tp as [H_tp1 H_tp2].
+  destruct H_tp2 as [H_tp2 H_tp3].
+  destruct H_decomposition as [t' [o]].
+  destruct H as [H_tEnd H_tSets].
+  (* We know that tp ∈ Tr∘s(P↓) ∩ Tr•s(a) *)
+  assert ((in_Traces_p tp (COMPILE_PROG P↓) s)
+       \/ (in_Traces_a tp a s)) as H_tp_in_Pa.
+  Case "Proof of tp ∈ Tr∘s(P↓) ∩ Tr•s(a)".
+  { destruct H_tSets as [HD|HD].
+    SCase "Left".
+    pose (trace_sets_closed_under_prefix_program 
+      tp ti (COMPILE_PROG P↓) s H_shp H_tp1 HD)
+      as H_prefix_closure.
+    left; apply H_prefix_closure.
+    SCase "Right".
+    pose (trace_sets_closed_under_prefix_context tp ti
+      a s H_sha H_tp1 HD)
+      as H_prefix_closure.
+    right; apply H_prefix_closure.
+  } 
+  (* tp is a strict prefix *)
+  assert (tp <> ti) as strict_prefix.
+  Case "Proof of distinction between tp and ti".
+  { unfold not. intro contra.
+    assert (H_shq := H_shQ).
+    apply shape_closed_under_compilation in H_shq.
+    pose (trace_composition tp s (COMPILE_PROG Q↓)
+      H_shq a H_sha) as t_composition. admit.
+  }
+Admitted.
+
+Definition secure_compartmentalizing_compilation : Prop :=
+  admit.
+
+Lemma SCC_isormorphism :
+  structured_full_abstraction ->
+  separate_compilation_correctness ->
+  secure_compartmentalizing_compilation.
 Proof.
 Admitted.
 
